vcheck.sh
@@ -2,6 +2,8 @@
 
 make="make -f $ISADK_DIR/Makefile $*"
 
+$make -C $ISADK_DIR/coq Isabelle.vo
+
 for d in `awk '/^-Q /{if($2!="."){print $2}}' _CoqProject`
 do
     $make -C $d
